Expr.v
@@ -9,9 +9,9 @@ Section Expr.
     {builtin : Type}.
 
   Inductive expr :=
-| valExpr : val -> expr
-| varExpr : var -> expr
-| appExpr : builtin -> list expr -> expr
+  | valExpr : builtin -> expr
+  | varExpr : var -> expr
+  | appExpr : expr -> expr -> expr
   .
 
   Program Instance exprS : Setoid expr :=
@@ -19,115 +19,64 @@ Section Expr.
       equiv := eq
     }.
 
-  Section ExprInductionPrinciple.
-    Variables (p : expr -> Prop) (Q : list expr -> Prop).
-
-    Hypothesis
-      (pval : forall val, p (valExpr val))
-      (pvar : forall var, p (varExpr var))
-      (papp0 : Q List.nil)
-      (papp1 : forall e, p e -> forall l, Q l -> Q (e :: l))
-      (papp : forall builtin l, Q l -> p (appExpr builtin l)).
-    
-    Fixpoint expr_ind_2 e : p e :=
-      match e as x return p x with
-        | valExpr val => pval val
-        | varExpr var => pvar var
-        | appExpr builtin l =>
-          papp builtin l ((fix dep_fold_right (l' : list expr) : Q l' :=
-                             match l' as x return Q x with
-                               | List.nil => papp0
-                               | e :: es => papp1 e (expr_ind_2 e) es (dep_fold_right es)
-                             end
-                          ) l)
-      end.
-  End ExprInductionPrinciple.
 
   Fixpoint exprFreeVars expr :=
     match expr with
       | valExpr _ => FVarSet.empty
       | varExpr var => FVarSet.singleton var
-      | appExpr builtin exprs =>  fold_right FVarSet.union FVarSet.empty (map exprFreeVars exprs)
+      | appExpr e1 e2 => FVarSet.union (exprFreeVars e1) (exprFreeVars e2)
     end
   .
 
 End Expr.
 
-
-Module Type BuiltInExpr (TT:TypeType) (AT:AddrType) (PT : PredType) (VT : ValType) (S : Store VT) (H : Heap TT AT PT VT).
-  Import TT AT PT VT.
+Module Type BuiltInExpr (VT : ValType) (S : Store VT).
   Parameter builtInExpr : Type.
   Parameter builtInExprS : Setoid builtInExpr.
-  Parameter appBIE : builtInExprS ~> listS valS ~~> H.tS ~~> S.tS ~~> optionS valS.
+  Parameter interpretBuiltInExpr : builtInExprS ~> S.tS ~~> maybeS VT.valS.
 End BuiltInExpr.
-  
-Module ExprModel (TT:TypeType) (AT:AddrType) (PT : PredType) (VT : ValType)  (S : Store VT) (H : Heap TT AT PT VT) (B : BuiltInExpr TT AT PT VT S H).
+
+Module ExprModel (VT : ValType)   (S : Store VT) (B: BuiltInExpr VT S).
   Import VT S B.
-  Definition expr := @expr val builtInExpr.
-  Instance exprS : Setoid expr := @exprS val builtInExpr.
+  Definition expr := @expr builtInExpr.
+  Instance exprS : Setoid expr := @exprS builtInExpr.
   Existing Instance maybe_Monad.
   Existing Instance monadFunctor.
   Existing Instance monad_Applicative.
-  Fixpoint _exprEval (h : H.t) (s : S.t ) (e : expr) : maybe val :=
+  Fixpoint _exprEval (s : S.t ) (e : expr) : maybe val :=
     match e with
-      | valExpr val => Some val 
+      | valExpr val => interpretBuiltInExpr @ val @ s
       | varExpr var => s [ var ]s
-      | appExpr b args =>
-        match (
-            fix _exprsEval (h : H.t) (s : S.t) (l : list expr) : option (list val) :=
-              match l with
-                | List.nil => ret @ @nil val
-                | e :: es => consS <$> _exprEval h s e <*> _exprsEval h s es
-              end) h s args with
-          | None => None
-          | Some l => appBIE @ b @ l @ h @ s
-        end
+      | appExpr e1 e2 => appVal <$> _exprEval s e1 <*> _exprEval s e2 >>= idS
     end.
   
-  Definition exprEval : H.tS ~> S.tS ~~> exprS ~~> optionS valS.
-    simple refine (
-             injF3 _exprEval _).
-    Lemma exprEval_1 :  Proper (equiv ==> equiv ==> equiv ==> equiv) _exprEval.
-    Proof.
-      autounfold. intros. simpl in H1. rewrite H1. clear H1 x1. generalize H H0. clear H H0. apply expr_ind_2 with (e:=y1) (Q:=fun es => allTrue (fun y1 => x == y -> x0 == y0 -> _exprEval x x0 y1 == _exprEval y y0 y1) es).
-      intros. simpl. reflexivity.
-      intros. simpl. equiv (x0 [var ]s) (y0 [var ]s). auto. 
-      compute. auto.
-      intros. unfold allTrue. rewrite map_cons.  rewrite fold_right_cons. split.
-      auto.
-      auto.
-      intros. unfold _exprEval. fold _exprEval. pose (_es:=(fix _exprsEval h (s : t) (l0 : list expr) {struct l0} :
-        option (list val) :=
-        match l0 with
-        | nil => ret @ @nil val
-        | e :: es => consS <$> _exprEval h s e <*> _exprsEval h s es
-        end)). fold _es. assert (_es x x0 l == _es y y0 l).  induction l.
-      simpl. constructor. 
-      unfold _es. fold _es. destruct H. rewrite (IHl H2). rewrite (H H0). reflexivity. auto.
-equiv (_es x x0 l) (_es y y0 l). simpl in H2. rewrite H0, H1, H2. reflexivity. 
-    Qed.
-    apply exprEval_1.  
-  Defined.
+  Instance exprEval_Proper :  Proper (equiv ==> equiv ==> equiv) _exprEval.
+  Proof.
+    autounfold. intros. simpl in H0. rewrite H0. clear H0 x0. generalize H. clear H. induction y0. 
+    - intros. simpl. rewrite H. reflexivity.
+    - intros. simpl. equiv (x [v ]s) (y [v ]s). auto. 
+    - intros. unfold _exprEval. fold _exprEval. evalproper. evalproper. evalproper. evalproper. evalproper. auto. auto. 
+  Qed.
   
-  Definition _exprsEval h s (es : list expr) : maybe (list val) :=  
-     mapM @ (exprEval @ h @ s) @ es.
+  Definition exprEval : S.tS ~> exprS ~~> optionS valS := injF2 _exprEval _.
   
-  Definition exprsEval : H.tS ~> tS ~~> listS exprS ~~> optionS (listS valS).
-    simple refine (    injF3 _exprsEval _).
-    Lemma exprsEval_1 : Proper (equiv ==> equiv ==> equiv ==> equiv) _exprsEval.
-    Proof.
-      repeat autounfold. intros. generalize H0 H1. clear H0 H1. apply list_ind_2 with (l1 := x1) (l2 := y1).
-      intros. constructor.
-      intros. inversion H2.
-      intros. inversion H2.
-      intros. inversion H2. unfold _exprsEval in *.  rewrite H6. rewrite H8. rewrite H. rewrite H1. reflexivity.
-    Qed.
-    apply exprsEval_1.
-  Defined.
+  Definition _exprsEval s (es : list expr) : maybe (list val) :=  
+     mapM @ (exprEval @ s) @ es.
   
-  Notation "⟦ e ⟧expr" := (fun s h => exprEval @ h @ s @ e)(at level 20).
-  Notation "⟦ es ⟧exprs" := (fun s h => exprsEval @ h @ s @ es) (at level 20).
+  Instance exprsEval_Proper : Proper (equiv ==> equiv ==> equiv) _exprsEval.
+  Proof.
+    repeat autounfold. intros. generalize H0. clear H0. apply list_ind_2 with (l1 := x0) (l2 := y0).
+    intros. constructor.
+    intros. inversion H1.
+    intros. inversion H1.
+    intros. inversion H1. unfold _exprsEval in *.  rewrite H5. rewrite H7. rewrite H. reflexivity.
+  Qed.
+  
+  Definition exprsEval : tS ~> listS exprS ~~> optionS (listS valS) := injF2 _exprsEval _.
+  
+  Notation "⟦ e ⟧expr" := (fun s => exprEval @ s @ e)(at level 20).
+  Notation "⟦ es ⟧exprs" := (fun s => exprsEval @ s @ es) (at level 20).
 
-  Definition exprEval' := cycle3S @ (cycle3S @ exprEval).
+  Definition exprEval' := flipS @ exprEval.
 
 End ExprModel.
