SQL/SQLSemantics.v
@@ -1,4 +1,4 @@
-Require Import Assert Command Definitions Algebra.Monoid Expr Algebra.SetoidCat Algebra.Maybe Tactics Algebra.ListUtils Algebra.Functor Algebra.Applicative Algebra.Alternative Algebra.FoldableFunctor Algebra.PairUtils Algebra.Maybe Algebra.Monad Algebra.Lens.Lens Utils SetoidUtils SQLStore SQLHeap SQL Lista Matrixp.
+Require Import Assert Command Definitions Algebra.Monoid Expr Algebra.SetoidCat Algebra.Maybe Tactics Algebra.ListUtils Algebra.Functor Algebra.Applicative Algebra.Alternative Algebra.FoldableFunctor Algebra.PairUtils Algebra.Maybe Algebra.Monad Algebra.Lens.Lens Utils SetoidUtils SQLStore SQLHeap SQL Lista Matrixp Pointed.
 Require Import Coq.Structures.DecidableTypeEx List SetoidClass PeanoNat FMapWeakList Basics.
 
 Existing Instance maybe_Monad.
@@ -7,23 +7,50 @@ Existing Instance monad_Applicative.
 
 Existing Instance sqlVal_Pointed.
 
-Module SQLBuiltInExpr (B : BuiltInExpr SQLTypeType SQLAddrType SQLPredType SQLValType SQLStore SQLHeap) <: BuiltInExpr SQLTypeType SQLAddrType SQLPredType SQLValType SQLStore SQLHeap.
+Definition _fromMaybe {A} {AS: Setoid A} {AP : Pointed A} (a : maybe A) := 
+  match a with
+    | None => point
+    | Some a => a
+  end
+.
+
+Instance _fromMaybe_Proper A AS AP : Proper (equiv ==> equiv) (@_fromMaybe A AS AP).
+Proof.
+  autounfold. intros. unfold _fromMaybe. matchequiv. auto. 
+Qed.
+
+Definition fromMaybe { A AS AP} := injF (@_fromMaybe A AS AP)  _.
+
+Instance fromMaybe_Pointed A AS AP : PointedFunction (@fromMaybe A AS AP).
+Proof.
+  split. reflexivity.
+Qed.
+
+Module SQLAsBuiltInExpr (B : BuiltInExpr SQLValType SQLStore) <: BuiltInExpr SQLValType SQLStore.
   Definition builtInExpr := sqlExpr B.builtInExpr.
   Instance builtInExprS : Setoid builtInExpr := sqlExprS B.builtInExpr.
-  Fixpoint sqlExprEval (s : store) (h : database) (e : builtInExpr) : option sqlVal :=
+  Fixpoint col (n : nat) (row : sqlVal) : option sqlVal :=
+    match row with
+      | vRow a b =>
+        match n with
+          | O => Some a
+          | S n1 => col n1 b
+        end
+      | _ => None
+    end
+  .
+  
+  Fixpoint sqlExprEval (s : store) (e : builtInExpr) : option sqlVal :=
     match e with
-      | sqlValExpr _ val => Some val
+      | sqlValExpr _ val => B.interpretBuiltInExpr @ val @ s
       | sqlVarExpr _ var => SQLStore.read @ var @ s 
       | sqlColExpr _ a colind =>
-        match sqlExprEval s h a with
-             | Some (vAddr (t, ri)) => cellGetter @ t @ ri @ colind @ h
+        match sqlExprEval s a with
+             | Some (vRow a b) => col colind (vRow a b) 
              | _ => None
         end
-      | sqlAppExpr _ builtin args =>
-        match sequence (map (sqlExprEval s h) args) with
-          | Some l => B.appBIE @ builtin @ l @ h @ s
-          | None => None
-        end
+      | sqlAppExpr _ e1 e2 =>
+        SQLValType.appVal <$> sqlExprEval s e1 <*> sqlExprEval s e2 >>= idS
     end
   .
 Ltac matchassertequiv := match goal with
@@ -33,141 +60,212 @@ Ltac matchdestruct := match goal with
             | |- _ (match ?a with _ => _ end) (match ?b with _ => _ end) => destruct a, b
                       end.
 
-Lemma sqlExprEval_Proper : Proper (equiv ==> equiv ==> equiv ==> equiv)
+Instance sqlExprEval_Proper : Proper (equiv ==> equiv ==> equiv)
                                  sqlExprEval.
     Proof.
-      autounfold. intros. simpl in H1. rewrite H1.
-      apply sqlExpr_ind_2 with (e:=y1) (Q:=fold_right (fun y1 p => sqlExprEval x x0 y1 == sqlExprEval y y0 y1 /\ p) True).
-      - simpl. reflexivity.
+      autounfold. intros. simpl in H0. rewrite H0. clear x0 H0.
+      induction y0.
+      - simpl. rewrite H. reflexivity.
       - intros. simpl. rewrite H. reflexivity.
-      - intros. simpl. matchequiv. matchequiv. inversion H4. inversion H4. simpl in H4. inversion H4. destruct s0. matchequiv. destruct m, m0. simpl in H5. simpl. matchassertequiv. rewrite H5. reflexivity.  matchdestruct.  simpl in H7. rewrite H7. reflexivity. inversion H7. inversion H7. reflexivity. 
-      - simpl.  auto.
-      - intros. split.
-        + rewritesr.
-        + auto.
-      - intros. unfold sqlExprEval.  fold sqlExprEval. matchassertequiv.
-        + induction l.
-          * simpl. reflexivity.
-          * rewrite map_cons. rewrite map_cons.
-            rewrite sequence_cons. rewrite sequence_cons. destruct H2. rewrite IHl. rewrite H2. reflexivity. apply H3.
-        + matchequiv. simpl in H3. rewrite H, H0, H3. reflexivity.
+      - intros. unfold sqlExprEval. fold sqlExprEval. evalproper. evalproper. evalproper. evalproper. evalproper. auto. auto. 
+      - simpl. matchequiv. simpl in H0. rewrite H0. reflexivity. 
     Qed.
     
-  Definition appBIE : builtInExprS ~> listS sqlValS ~~> SQLHeap.tS ~~> SQLStore.tS ~~> maybeS sqlValS.
-    refine (injF4 (fun e _ h s => sqlExprEval s h e) _).
-    Lemma sqlExprEval_1 : Proper (equiv ==> equiv ==> equiv ==> equiv ==> equiv)
-                                 (fun (e : builtInExpr) (_ : list sqlVal) h (s : store) => sqlExprEval s h e).
-    Proof.
-      autounfold. intros. simpl in H. rewrite H.
-      apply sqlExpr_ind_2 with (e:=y) (Q:=fold_right (fun y p => sqlExprEval x2 x1 y == sqlExprEval y2 y1 y /\ p) True).
-      - simpl. reflexivity.
-      - intros. simpl. rewrite H2. reflexivity.
-      - intros. simpl. matchequiv. matchequiv.  inversion H5. inversion H5. simpl in H3. inversion H3. destruct s0. matchassertequiv. rewritesr. matchdestruct. destruct m, m0. simpl. simpl in H6. matchassertequiv. rewrite H6. reflexivity. matchdestruct. simpl in H8. rewrite H8. reflexivity. inversion H8. inversion H8. reflexivity. inversion H6. inversion H6. reflexivity. 
-      - simpl.  auto.
-      - intros. split.
-        + rewritesr.
-        + auto.
-      - intros. unfold sqlExprEval.  fold sqlExprEval. matchassertequiv.
-        + induction l.
-          * simpl. reflexivity.
-          * rewrite map_cons. rewrite map_cons.
-            rewrite sequence_cons. rewrite sequence_cons. destruct H3. rewrite IHl. rewrite H3. reflexivity. apply H4.
-        + matchequiv. simpl in H4. rewrite H1, H2, H4. reflexivity.
-    Qed.
-    apply sqlExprEval_1.
-  Defined.
-  
-End SQLBuiltInExpr.
+    Definition interpretBuiltInExpr : builtInExprS ~> SQLStore.tS ~~> maybeS sqlValS := flipS @ (injF2 sqlExprEval _).
+    
+End SQLAsBuiltInExpr.
 
-Module SQLBuiltInFormula (BIE : BuiltInExpr SQLTypeType SQLAddrType SQLPredType SQLValType SQLStore SQLHeap) (BIF : BuiltInFormula SQLTypeType SQLAddrType SQLPredType SQLValType SQLStore SQLHeap) <: BuiltInFormula SQLTypeType SQLAddrType SQLPredType SQLValType SQLStore SQLHeap.
-  Module SQLBIE := SQLBuiltInExpr BIE.
-  Definition builtInFormula := sqlFormula BIE.builtInExpr BIF.builtInFormula.
-  Instance builtInFormulaS : Setoid builtInFormula := sqlFormulaS BIE.builtInExpr BIF.builtInFormula.
-  Definition storeToRow (rets : list (sqlExpr BIE.builtInExpr)) (s : store) (h : database) : maybe row :=
-    listaConsS <$> (sequence (map (fun (e : sqlExpr BIE.builtInExpr) =>
-                                       SQLBIE.sqlExprEval s h e
+(* builtInFormula *)
+Module Type SQLBuiltInFormula.
+  Parameter builtInCommand : Type.
+  Parameter builtInCommandS : Setoid builtInCommand.
+  Parameter appSQLBuiltInFormula : builtInCommandS ~> sqlValS ~~> sqlValS ~~> maybeS unitS.
+End SQLBuiltInFormula.
+
+(* SQL as builtInCommand *)
+Module SQLAsBuiltInCommand (B : BuiltInExpr SQLValType SQLStore ) (BIC : SQLBuiltInFormula ) <: BuiltInCommand SQLTypeType SQLAddrType SQLPredType SQLValType SQLStore SQLHeap.
+  Module SQLB := SQLAsBuiltInExpr B.
+  Definition builtInFormula := sqlFormula B.builtInExpr BIC.builtInCommand.
+  Instance builtInFormulaS : Setoid builtInFormula := sqlFormulaS B.builtInExpr BIC.builtInCommand.
+  Definition builtInCommand := sqlStmt B.builtInExpr BIC.builtInCommand.
+  Instance builtInCommandS : Setoid builtInCommand := sqlStmtS B.builtInExpr BIC.builtInCommand.
+
+  Instance storeProd_Proper : Proper (equiv ==> equiv ==> equiv) storeProd.
+  Proof.
+    solve_properS storeProd.
+  Qed.
+
+  Definition storeProdS := injF2 storeProd _.
+  
+  Definition restrictStore (rets : list (sqlExpr B.builtInExpr * var)) (s : store) : maybe store :=
+    fold_rightS @ storeProdS @ SQLStore.emptyStore
+                <$> (sequence (map (fun (e : sqlExpr B.builtInExpr * var) =>
+                                      SQLStore.update @ (snd e)
+                                                      <$> (SQLB.sqlExprEval s (fst e))
+                                                      <*> pure @ SQLStore.emptyStore 
                    ) rets)) .
-
   
-    Fixpoint sqlFormEval (s : store) (m : database) (form: builtInFormula) : list SQLStore.t :=
-      match form with
-        | sqlBuiltInFormula _ _ builtin args =>
-          match sequenceS @ (mapS @ (cycle3S @ SQLBIE.appBIE @ nil @ s) @ args) with
-            | Some l => BIF.appBIF @ builtin @ l @ m @ s
-            | None => nil
-          end
-        | sqlAnd _ _ form1 form2 =>
-          concat (map (fun s => sqlFormEval s m form2) (sqlFormEval s m form1))
-        | sqlOr _ _ form1 form2 =>
-          sqlFormEval s m form1 ++ sqlFormEval s m form2
-        | sqlNot _ _ form1 =>
-          if null (sqlFormEval s m form1) then
-            s :: nil
-          else
-            nil
-        | sqlExists _ _ sql =>
-          if null (sqlReduce s m sql) then
-            nil
-          else
-            s :: nil
-      end
-    with
-    sqlReduce (s : store) (m : database) (sql1 : sql BIE.builtInExpr BIF.builtInFormula) : list row :=
-      match sql1 with
-        | sqlQuery _ _ rets tabs form =>
-          
-          let ss := fold_left
-            storesProd
-            (map (fun tab : sqlTableExpr BIE.builtInExpr BIF.builtInFormula * var =>
-                    let (te, var) := tab in
-                    map (fun r => SQLStore.update @ var @ (vRow r) @ SQLStore.emptyStore) (map listOfLista (sqlTableExprEval s m te))) tabs) 
-            (s :: List.nil) in
-          let filtered := concat (map (fun s => sqlFormEval s m form) ss) in 
-          list_filter'  (map (storeToRow rets) filtered)
-      end
-    with
-    sqlTableExprEval (s : store) (m : database) (te : sqlTableExpr BIE.builtInExpr BIF.builtInFormula) : list row :=
-      match te with
-        | sqlTable _ _ tab => match (nth_error m tab) with
-                            | Some tab => lista_filter' (rows @ tab)
-                            | None => nil
-                          end
-        | sqlSelect _ _ sql1 => sqlReduce s m sql1
-      end
-    .
+  Definition getTableRows (m : database) (tab : nat) : lista (maybe row) := 
+    match (nth_error m tab) with
+      | Some tab => rows @ tab
+      | None => listaCons _ nil
+    end
+  .
 
-    Existing Instance sqlTableExprS.
+  Definition sqlTableExprEval (m : database) (tab : nat)  : list row :=  lista_filter' (getTableRows m tab).
 
-    Instance vRow_Proper : Proper (equiv ==> equiv) vRow.
-    Proof.
-      autounfold. intros. simpl in *. rewrite H. 
-    Instance sqlFormEval_Proper : Proper (equiv ==> equiv ==> equiv ==> equiv) sqlFormEval.
-    Proof.
-      autounfold. intros. generalize x y H H1. clear x y H H1.
-      refine (sqlFormula_ind_2 _ _
-      (fun x1 y1 => forall x y : store,
-   x == y -> x1 == y1 -> sqlFormEval x x0 x1 == sqlFormEval y y0 y1)
-      (fun q1 q2 => forall x y : store,
-                         x == y -> @equiv (sql _ _) (sqlS _ _) q1 q2 -> sqlReduce x x0 q1 == sqlReduce y y0 q2)
-      (fun tel1 tel2 => forall x y : store,
-                             x == y -> tel1 == tel2 -> fold_right and True (list_zipWith_not_proper (fun vt1 vt2 =>
-                                                                                             match vt1, vt2 with
-                                                                                               | (te1, v1), (te2, v2) => sqlTableExprEval x x0 te1 == sqlTableExprEval y y0 te2
-                                                                                             end
-                                                                                          ) tel1 tel2))
-      (fun te1 te2 =>
-            forall x y : store,
-              x == y -> te1 == te2 -> sqlTableExprEval x x0 te1 == sqlTableExprEval y y0 te2)
+  Definition listaToVRow (la : lista sqlVal) :=
+    match la with
+      | listaCons _ l => fold_right (fun a l =>
+                                       match a with
+                                         | vNil =>
+                                           match l with
+                                             | vNil => vNil
+                                             | _ => vRow a l
+                                           end
+                                         | _ => vRow a l
+                                       end) vNil l
+    end
+  .
+
+  Instance listaToVRow_Proper : Proper (equiv ==> equiv) listaToVRow.
+  Proof.
+    autounfold. intros. destruct x,y. generalize H. clear H. apply list_ind_2 with (l1:=l) (l2:=l0).
+    - intros. reflexivity.
+    - intros. inversion H0. simpl in H1. rewrite H1. unfold listaToVRow.  rewrite fold_right_cons. fold (listaToVRow (listaCons _ b)).      rewrite <- H.  simpl. reflexivity. auto. 
+    - intros. inversion H0. simpl in H1. rewrite H1. unfold listaToVRow.  rewrite fold_right_cons. fold (listaToVRow (listaCons _ b)).      rewrite H.  simpl. reflexivity. auto. 
+    - intros. unfold listaToVRow. rewrite fold_right_cons. rewrite fold_right_cons. fold (listaToVRow (listaCons _ b)). fold (listaToVRow (listaCons _ d)).  inversion H0. rewrite H.  clear H. destruct a, c. 
+      inversion H1. reflexivity.
+      inversion H1.
+      inversion H1.
+      inversion H1.
+      inversion H1.
+      inversion H1.
+      inversion H1. reflexivity.
+      inversion H1.
+      inversion H1.
+      inversion H1.
+      inversion H1. 
+      inversion H1.
+      reflexivity. 
+      inversion H1.
+      inversion H1.
+      inversion H1.
+      inversion H1.
+      inversion H1.
+      inversion H1. reflexivity.
+      inversion H1.
+      inversion H1.
+      inversion H1.
+      inversion H1.
+      inversion H1.
+      rewrite H1. reflexivity.
+      auto.
+  Qed.
+
+  Definition _sqlValToStorableVal (a : maybe sqlVal) := 
+    match a with
+      | None => None
+      | Some a => if SQLValType.storable a then Some a else None
+    end
+  .
+
+
+  Instance _sqlValToStorableVal_Proper : Proper (equiv ==> equiv) _sqlValToStorableVal.
+  Proof.
+    autounfold. intros. unfold _sqlValToStorableVal. matchequiv. simpl in *. rewrite H. reflexivity.
+  Qed.
+
+  Definition sqlValToStorableVal := injF _sqlValToStorableVal _.
+
+  Instance sqlValToStorableVal_Pointed : PointedFunction sqlValToStorableVal.
+  Proof.
+    split. reflexivity.
+  Qed.
+
+  Definition _storeToRow (s : store) : row :=
+    lista_mapS fromMaybe @ (lista_mapS sqlValToStorableVal @ s)
+  .
+
+  Instance _storeToRow_Proper : Proper (equiv ==> equiv) _storeToRow.
+  Proof.
+    autounfold. intros.  destruct x,y. unfold _storeToRow.  rewritesr.
+  Qed.  
+
+  Definition storeToRow := injF _storeToRow _.
+
+  Definition _rowStore (var1 : var) (r : row) := SQLStore.update @ var1 @ (listaToVRow r) @ SQLStore.emptyStore.
+
+  Instance _rowStore_Proper : Proper (equiv ==> equiv ==> equiv) _rowStore.
+  Proof.
+    solve_properS _rowStore.
+  Qed.
+
+  Definition rowStore := injF2 _rowStore _.
+  
+  Definition rowsToStores (var1 : var) (rows : list row) := mapS @ (rowStore @ var1) @ rows.
+  
+  Fixpoint sqlFormEval (s : store) (m : database) (form: builtInFormula) : list SQLStore.t :=
+    match form with
+      | sqlBuiltIn _ _ builtin e1 e2 =>
+        match SQLB.interpretBuiltInExpr @ e1 @ s, SQLB.interpretBuiltInExpr @ e2 @ s with
+          | Some v1, Some v2 =>
+            match BIC.appSQLBuiltInFormula @ builtin @ v1 @ v2 with
+              | Some _ => s :: nil
+              | _ => nil
+            end
+          | _, _ => nil
+        end
+      | sqlAnd _ _ form1 form2 =>
+        concat (map (fun s => sqlFormEval s m form2) (sqlFormEval s m form1))
+      | sqlOr _ _ form1 form2 =>
+        sqlFormEval s m form1 ++ sqlFormEval s m form2
+      | sqlNot _ _ form1 =>
+        if null (sqlFormEval s m form1) then
+          s :: nil
+        else
+          nil
+      | sqlExists _ _ sql =>
+        if null (sqlReduce s m sql) then
+          nil
+        else
+          s :: nil
+    end
+  with
+  sqlReduce (s : store) (m : database) (sql1 : sql B.builtInExpr BIC.builtInCommand) : list store :=
+    match sql1 with
+      | sqlQuery _ _ rets tabs form =>        
+        let ss := fold_left
+                    storesProd
+                    (map (fun tab : nat * var =>
+                            let (te, var) := tab in
+                            rowsToStores var (sqlTableExprEval m te)) tabs) 
+                    (s :: List.nil) in
+        let filtered := concat (map (fun s => sqlFormEval s m form) ss) in 
+        list_filter'  (map (restrictStore rets) filtered)
+    end
+  .
+
+  Instance vRow_Proper : Proper (equiv ==> equiv ==> equiv) vRow.
+  Proof.
+    solve_proper. 
+  Qed.
+
+  Existing Instance sqlS.
+  Instance sqlFormEval_Proper : Proper (equiv ==> equiv ==> equiv ==> equiv) sqlFormEval.
+  Proof.
+    autounfold. intros. generalize x y H H1. clear x y H H1.
+    refine (sqlFormula_ind_2 B.builtInExpr BIC.builtInCommand (fun x1 y1=>forall x y : store,
+   x == y -> x1 == y1 -> sqlFormEval x x0 x1 == sqlFormEval y y0 y1) (fun x1 y1=>forall x y : store,
+   x == y -> x1 == y1 -> sqlReduce x x0 x1 == sqlReduce y y0 y1) 
       _ _ _ _ _
       _ _ _ _ _
       _ _ _ _ _
       _ _ _ _ _
       _ _ _ _ _
       _
-      _ _ _ _
-      _ _ _ _
       x1 y1).
-      - intros.  unfold sqlFormEval.  inversion H1. matchequiv. simpl in H2. rewrite H, H0, H2. reflexivity.
+    - intros.  unfold sqlFormEval.  inversion H1. matchequiv. matchequiv. matchequiv. rewrite H.  reflexivity. 
       - intros.  inversion H1.
       - intros. inversion H1.
       - intros. inversion H1.
@@ -214,30 +312,13 @@ Module SQLBuiltInFormula (BIE : BuiltInExpr SQLTypeType SQLAddrType SQLPredType 
         + inversion H3.
         + inversion H3.
         + rewritesr. 
-      - intros. inversion H3. Opaque equiv. simpl.  Transparent equiv.
+      - intros. inversion H2. clear H2. Opaque equiv. simpl. Transparent equiv.
         apply list_filter'_Proper. apply map_Proper.
         + autounfold. intros. unfold storeToRow. evalproper. apply sequence_Proper. apply map_Proper.
-          * autounfold. intros. 
-            match goal with
-              | |- match ?a with _ => _ end == match ?b with _ => _ end => assert (a== b)
-            end.
-            apply SQLBIE.sqlExprEval_Proper. auto. auto.
-            match goal with
-              | |- match ?a with _ => _ end == match ?b with _ => _ end => destruct a, b
-            end.
-            {
-              simpl in H9. all_cases.  inversion H9. inversion H9. inversion H9. inversion H9.
-            }
-            {
-              inversion H9.
-            }
-            {
-              inversion H9.
-            }
-            reflexivity.
+          * autounfold. intros. evalproper. rewritesr. 
           * reflexivity.
         + apply concat_Proper.  apply map_Proper.
-          * autounfold. intros. rewrite <- H7 at 1. apply H1. auto. auto.
+          * autounfold. intros. rewrite <- H6 at 1. apply H. auto. auto.
           * apply fold_left_Proper.
             {
               autounfold. intros. unfold storesProd. apply concat_Proper. apply map_Proper.
@@ -255,37 +336,227 @@ Module SQLBuiltInFormula (BIE : BuiltInExpr SQLTypeType SQLAddrType SQLPredType 
               }
             }
             {
-              clear H. refine (map_Proper (fun tab : sqlTableExpr BIE.builtInExpr BIF.builtInFormula * var =>
-      let (te, var) := tab in
-      map
-        (fun r : list sqlVal =>
-         listaCons (option sqlVal) (lista_update0 var nil (Some (vRow r))))
-        (map listOfLista (sqlTableExprEval x x0 te))) (fun tab : sqlTableExpr BIE.builtInExpr BIF.builtInFormula * var =>
-      let (te, var) := tab in
-      map
-        (fun r : list sqlVal =>
-         listaCons (option sqlVal) (lista_update0 var nil (Some (vRow r))))
-        (map listOfLista (sqlTableExprEval y y0 te))) _ tel2 tel2 _).
+              clear H. apply map_Proper;[|reflexivity]. autounfold. intros. destruct x2, y2. destruct H. apply map_Proper.
               {
-                autounfold. intros. repeat rewrite let_intro. apply map_Proper. autounfold. intros. apply listaCons_Proper. apply lista_update0_Proper. 
-                apply (@snd_Proper (sqlTableExpr BIE.builtInExpr BIF.builtInFormula) _ equiv _). auto. reflexivity. apply Some_Proper. apply vRow_Proper. rewrite H. unfold equiv in H.  simpl in H. 
-            rewrite H4, H8.
+                autounfold. intros. apply listaCons_Proper. apply lista_update0_Proper. auto. reflexivity. apply Some_Proper. apply listaToVRow_Proper. auto.
+              }
+              {
+                unfold sqlTableExprEval. apply lista_filter'_Proper. unfold getTableRows. matchequiv. simpl in H3. rewrite H3. reflexivity.
+              }
+            }
+            {
+              rewritesr.
+            }
+  Qed.
 
-            matchequiv. rewritesr. reflexivity. simpl. fold fold_left. _cons.
-      - intros. inversion H1.
-      - intros. inversion H1.
-      - intros. inversion H1.
-      - intros. inversion H1.
-      - intros. inversion H1.
+  Instance restrictStore_Proper : Proper (equiv ==> equiv ==> equiv) restrictStore.
+  Proof.
+    autounfold. intros.  unfold restrictStore. evalproper. apply sequence_Proper.  apply map_Proper. autounfold. intros. rewrite H0, H1. reflexivity. auto.
+  Qed.
+  
+  Instance storesProd_Proper : Proper (equiv ==> equiv ==> equiv) storesProd.
+  Proof.
+    autounfold. intros.  unfold storesProd. apply concat_Proper.  apply map_Proper. autounfold. intros. apply map_Proper. autounfold. intros. apply storeProd_Proper. auto. auto. auto. auto. 
+  Qed.
+  
+  Instance rowsToStores_Proper : Proper (equiv ==> equiv ==> equiv) rowsToStores.
+  Proof.
+    autounfold. intros.  unfold rowsToStores. rewritesr. 
+  Qed.
 
-    Definition appBIF : sqlFormulaS ~> listS sqlValS ~~> databaseS ~~> storeS ~~> listS storeS :=
-  constS _ @ (constS _ @ (constS _ @ constS _ @ nil)).
-End SQLBuiltInFormula.
+  Instance getTableRows_Proper : Proper (equiv ==> equiv ==> equiv) getTableRows.
+  Proof.
+    autounfold. intros.  unfold getTableRows. matchequiv. simpl in H1. rewrite H1. reflexivity. 
+  Qed.
+
+  Instance sqlTableExprEval_Proper : Proper (equiv ==> equiv ==> equiv) sqlTableExprEval.
+  Proof.
+    autounfold. intros. unfold sqlTableExprEval. apply lista_filter'_Proper. apply getTableRows_Proper. auto. auto.
+  Qed.
+  
+  Instance sqlReduce_Proper : Proper (equiv ==> equiv ==> equiv ==> equiv) sqlReduce.
+  Proof.
+    autounfold. intros. destruct x1, y1. rewrite H1. clear H1. Opaque equiv. simpl. Transparent equiv. apply list_filter'_Proper. apply map_Proper. autounfold. intros. apply restrictStore_Proper. reflexivity. auto. apply concat_Proper. apply map_Proper. autounfold. intros. apply sqlFormEval_Proper. auto. auto. reflexivity. apply fold_left_Proper. autounfold. intros. apply storesProd_Proper. auto. auto. apply map_Proper. autounfold. intros. destruct x1, y1. destruct H1.  apply rowsToStores_Proper. auto. apply sqlTableExprEval_Proper. auto. auto. reflexivity. constructor.  auto. reflexivity.
+  Qed.
+  
+  Definition insertRows (table : nat) (rows : list row) (m : database) : maybe database := rowsSetter @ table <$> (lista_mergeS <$> rowsGetter @ table @ m <*> pure @ rows) <*> pure @ m.
+
+  Definition deleteRow (table : nat) (ri : nat) (m : database) : maybe database := rowsSetter @ table <$> (lista_deleteS @ ri <$> rowsGetter @ table @ m) <*> pure @ m.
+
+  Definition updateRowS  : natS ~> natS ~~> natS ~~> sqlValS ~~> databaseS ~~> databaseS := cellSetter.
+
+  Definition _interpretBuiltInCommand0 (comm : builtInCommand) (m : database) (s : store) : database * list store :=
+    match comm with
+      | sqlQueryStmt _ _ sql => (m, sqlReduce s m sql)
+      | sqlInsertStmt _ _ table sql =>
+        match sql with
+          | sqlQuery _ _ rets _ _ =>
+            let cols := map snd rets in
+            let stores := sqlReduce s m sql in
+            let rows := mapS @ storeToRow @ stores in
+            match insertRows table rows m with
+              | None => (m, nil)
+              | Some m' => (m', s :: nil)
+            end
+        end
+      | sqlDeleteStmt _ _ table var1 form =>
+        let rows := getTableRows m table in
+        let storesi := mapS @ (idS *** rowStore @ var1) @ (lista_filter_indexS' @ rows) in
+        let m' := fold_right (fun ris m' =>
+                                match ris with
+                                  | (i, s) =>
+                                    match sqlFormEval s m' form with
+                                      | nil => m'
+                                      | _ =>
+                                        match deleteRow table i m' with
+                                          | None => m'
+                                          | Some m'' => m''
+                                        end
+                                    end
+                                end) m storesi in
+        (m', s::nil)
+      | sqlUpdateStmt _ _ table var1 updates form =>
+        let rows := getTableRows m table in
+        let storesi := mapS @ (idS *** rowStore @ var1) @ (lista_filter_indexS' @ rows) in
+        let m' := fold_right (fun ris m' =>
+                                match ris with
+                                  | (i, s) =>
+                                    match sqlFormEval s m' form with
+                                      | nil => m'
+                                      | _ =>
+                                        fold_right (fun update m'' =>
+                                               match update with
+                                                 | (c, e) =>
+                                                   match SQLB.sqlExprEval s e with
+                                                     | None => m''
+                                                     | Some val => updateRowS @ table @ i @ c @ val @ m''
+                                                   end
+                                               end) m' updates
+                                    end
+                                end) m storesi in
+        (m', s::nil)
+    end
+  .
+
+  Instance _interpretBuiltInCommand0_Proper : Proper (equiv ==> equiv ==> equiv ==> equiv) _interpretBuiltInCommand0.
+  Proof.
+    autounfold. intros. unfold _interpretBuiltInCommand0.  destruct x, y.
+    - split. auto. simpl in H. inversion H. apply sqlReduce_Proper. auto. auto. reflexivity.
+    - inversion H.
+    - inversion H.
+    - inversion H.
+    - inversion H.
+    - inversion H. destruct s0. assertequiv. unfold insertRows. rewritesr. matchequiv. simpl in H2. split. auto. constructor. auto. reflexivity. split. auto. reflexivity. 
+    - inversion H.
+    - inversion H.
+    - inversion H.
+    - inversion H.
+    - inversion H. split. apply fold_right_Proper. autounfold. intros. destruct x, y. destruct H2. matchequiv. auto. apply fold_right_Proper. autounfold. intros. destruct x, y. destruct H10. assertequiv. apply SQLB.sqlExprEval_Proper. auto. auto. matchequiv. simpl in H13. rewritesr. auto. auto. reflexivity. auto. rewritesr. rewritesr. 
+    - inversion H.
+    - inversion H.
+    - inversion H.
+    - inversion H.
+    - inversion H. split. apply fold_right_Proper. autounfold. intros. destruct x, y. destruct H2. matchequiv. auto. assertequiv. unfold deleteRow. rewritesr. matchequiv. simpl in H9. auto. auto. auto. rewritesr. rewritesr. 
+  Qed.
+  
+  Definition interpretBuiltInCommand0 : builtInCommandS ~> databaseS ~~> storeS ~~> databaseS ~*~ listS storeS :=
+    injF3 _interpretBuiltInCommand0 _.
+
+  Module TS := Types SQLTypeType SQLAddrType SQLPredType SQLValType SQLStore SQLHeap.
+
+  Existing Instance list_Foldable.
+  Existing Instance StoreHeap.sh_Alternative.
+  Existing Instance TS.state_Monad.
+  Existing Instance alternative_Monoid.
+  Existing Instance monad_Applicative.
+  
+  Definition _branchStores (ss : list store) : TS.state unit := fold @ (mapS @ StoreHeap.putStore @ ss).
+  Instance _branchStores_Proper : Proper (equiv ==> equiv) _branchStores.
+  Proof.
+    solve_properS _branchStores.
+  Qed.
+
+  Definition branchStores := injF _branchStores _.
+
+  Definition _interpretBuiltInCommand (comm : builtInCommand) : TS.state unit.
+    refine (
+    (interpretBuiltInCommand0
+      @ comm
+      <$> StoreHeap.getHeap
+      <*> StoreHeap.getStore) >>= injF (fun mss => match mss with
+                                                       | (m, ss) =>
+                                                         StoreHeap.putHeap @ m >>
+                                                                           branchStores @ ss
+                                                   end) _).
+    apply TS.state_Monad. 
+    Lemma _interpretBuiltInCommand_1 : Proper (equiv ==> equiv)
+     (fun mss : SQLHeap.t * list store =>
+        let (m, ss) := mss in StoreHeap.putHeap @ m >> branchStores @ ss).
+    Proof.
+      autounfold. intros. destruct x,y.  destruct H. rewritesr.
+    Qed.
+    apply _interpretBuiltInCommand_1.
+  Defined.
+  
+  Instance _interpretBuiltInCommand_Proper : Proper (equiv ==> equiv) _interpretBuiltInCommand.
+  Proof.
+    autounfold. intros. rewritesr. 
+  Qed.
+
+  Definition interpretBuiltInCommand : builtInCommandS ~> TS.stateS unitS :=
+    injF _interpretBuiltInCommand _.
+
+  Fixpoint sqlExprFreeVars (e : sqlExpr B.builtInExpr) :=
+    match e with
+      | sqlValExpr _ _ => FVarSet.empty
+      | sqlVarExpr _ v => FVarSet.singleton v
+      | sqlColExpr _ v _ => sqlExprFreeVars v
+      | sqlAppExpr _ e1 e2 => FVarSet.union (sqlExprFreeVars e1) (sqlExprFreeVars e2)
+    end
+  .
+  
+  Fixpoint freeVars (comm : builtInFormula) :=
+    match comm with
+      | sqlBuiltIn _ _ builtin e1 e2 =>
+        FVarSet.union (sqlExprFreeVars  e1) (sqlExprFreeVars  e2)
+      | sqlAnd _ _ form1 form2 =>
+        FVarSet.union (freeVars form1) (freeVars form2)
+      | sqlOr _ _ form1 form2 =>
+        FVarSet.union (freeVars form1) (freeVars form2)
+      | sqlNot _ _ form1 =>
+        freeVars form1
+      | sqlExists _ _ sql =>
+        sqlFreeVars sql
+    end
+  with
+  sqlFreeVars (s : sql B.builtInExpr BIC.builtInCommand) :=
+    match s with
+      | sqlQuery _ _ _ _ s1 => freeVars s1
+    end
+  .
+
+  Instance freeVars_Proper : Proper (equiv ==> equiv) freeVars.
+  Proof.
+    solve_properS freeVars.
+  Qed.
+
+  Definition _freeVarsBuiltInCommand (comm : builtInCommand) :=
+    match comm with
+      | sqlQueryStmt _ _ (sqlQuery _ _ _ _ form) =>
+        freeVars form
+      | sqlInsertStmt _ _ _ sql =>
+        sqlFreeVars sql
+      | sqlUpdateStmt _ _ _ _ _ form =>
+        freeVars form
+      | sqlDeleteStmt _ _ _ _ form =>
+        freeVars form
+    end
+  .
+
+  Definition freeVarsBuiltInCommand := injF _freeVarsBuiltInCommand _.
+End SQLAsBuiltInCommand.
       
-Module SQLModel .
-  (* SQL as builtInFormula and builtInCommand *)
   
 
 
     
-End SQLModel.
