Definitions.v
@@ -49,6 +49,8 @@ End TypeType.
 Module Type ValType.
   Parameter val : Type.
   Parameter valS : Setoid val.
+  Parameter storableS : valS ~> boolS.
+  Parameter appVal : valS ~> valS ~~> maybeS valS.
   Axiom equiv_dec : forall val1 val2, {val1 == val2} + {~ val1 == val2}.
 End ValType.
 
